state-plift changes

theory/Utils/StateT.v
@@ -30,20 +30,26 @@ Definition liftT {S M} `{Monad M} {A} (m : M A) : StateT S M A :=
     fun st =>
     a <- m ;; mreturn (a, st).
 
-Definition state_plift {S} {M} `{Monad M} `{PredLift M} {X} (Pre Post : S -> Prop) (P : X -> Prop) :
+Definition state_plift {S} {M} `{Monad M} `{PredLift M} {X} (Pre Post : S -> Prop) (P : X -> Prop) (R : X -> S -> Prop) :
   StateT S M X -> Prop :=
   fun mx =>
-    forall s, Pre s -> plift (fun '(x, s') => P x /\ Post s') (mx s).
+    forall s, Pre s -> plift (fun '(x, s') => P x /\ R x s' /\ Post s') (mx s).
+
+Definition triv {X} : X -> Prop :=
+  fun _ => True.
+
+Definition triv2 {X Y} : X -> Y -> Prop :=
+  fun _ _ => True.
 
 (*
  * state_prob_bind is analogous to the sequencing rule in Hoare Logic
  *)
 Lemma state_plift_bind {S X Y} {M} `{Monad M} `{PredLift M} {Pre : S -> Prop}
-      (Mid : S -> Prop) {Post : S -> Prop} (P: X -> Prop) {Q: Y -> Prop}
+      (Mid : S -> Prop) {Post : S -> Prop} (P: X -> Prop) {Q: Y -> Prop} {R : X -> S -> Prop} {T : Y -> S -> Prop}
       {mx : StateT S M X} {f : X -> StateT S M Y} : 
-  state_plift Pre Mid P mx ->
-  (forall x, P x -> state_plift Mid Post Q (f x)) ->
-  state_plift Pre Post Q (mbind mx f).
+  state_plift Pre Mid P R mx ->
+  (forall x, P x -> state_plift Mid Post Q T (f x)) ->
+  state_plift Pre Post Q T (mbind mx f).
 Proof.
   intros.
   unfold state_plift. intros.
@@ -54,52 +60,52 @@ Proof.
 Qed.
 
 Lemma state_plift_ret {S X} {M} `{Monad M} `{PredLift M} {Pre : S -> Prop} {P : X -> Prop} {x : X}:
-  P x -> state_plift Pre Pre P (mreturn x).
+  P x -> state_plift Pre Pre P triv2 (mreturn x).
 Proof.
   intros.
   unfold state_plift. intros.
   apply plift_ret.
-  split; auto.
+  repeat split; auto.
 Qed.
 
 Lemma state_plift_get {S} {M} `{Monad M} `{PredLift M} {Pre : S-> Prop} :
-  state_plift Pre Pre Pre get.
+  state_plift Pre Pre Pre triv2 get.
 Proof.
   intros s Hs.
   apply plift_ret.
-  split; auto.
+  repeat split; auto.
 Qed.
 
 Lemma state_plift_put {S} {M} `{PredLift M} {Pre Pre' : S -> Prop} : forall s,
-  Pre' s -> state_plift Pre Pre' (fun _ => True) (put s).
+  Pre' s -> state_plift Pre Pre' triv triv2 (put s).
 Proof.
   intros s Hs ? ?.
   apply plift_ret.
-  split; auto.
+  repeat split; auto.
 Qed.
 
 Lemma state_plift_liftT {S} {M} `{PredLift M} {Pre : S -> Prop}
   {X} {P : X -> Prop} : forall (m : M X),
   plift P m ->
-  state_plift Pre Pre P (liftT m).
+  state_plift Pre Pre P triv2 (liftT m).
 Proof.
   intros m Hm.
   intros s Hs.
   eapply plift_bind; eauto.
   intros x Hx.
   apply plift_ret.
-  split; auto.
+  repeat split; auto.
 Qed.
 
 Lemma state_plift_weaken {S} {M} `{PredLift M} {X}
   {Pre : S -> Prop} (Post : S -> Prop) {Post' : S -> Prop}
-  (P : X -> Prop) :
+  (P : X -> Prop) (R : X -> S -> Prop) :
   has_weakening M -> forall m,
   (forall s, Post s -> Post' s) ->
-  state_plift Pre Post P m ->
-  state_plift Pre Post' P m.
+  state_plift Pre Post P R m ->
+  state_plift Pre Post' P R m.
 Proof.
   intros HM m HPostPost' Hm s Hs.
   eapply HM; [| apply Hm; auto].
-  intros [x s'] [Hx Hs']; auto.
+  intros [x s'] [Hx [Hs' Hxs']]; auto.
 Qed.
